Drop visited_coherent invariant — derivable from done_id_coherent + valid d
Removes the existence-style [visited_coherent m d] ("∀ γ, d !! γ ≠ None →
∃ n, m !! γ is done/finished n") from visited_mapg_auth and the four
update predicates, since it follows from [done_id_coherent] together with
[✓ d] (every valid agree element is some [to_agree n] via to_agree_uninj).

Adds a derivation lemma [done_id_visited_coherent] for callers that still
need the existence form. Refactors visited_reached_done_invalid and
pending_set_remove to use done_id_coherent / Hdid directly.

theories/examples/susp_correctness/resource_algebras.v
@@ -56,17 +56,31 @@ Section visited_map_res.
   Definition penset_frag (γs : gset gname) : iProp Σ :=
     own pending_set_name (◯ GSet γs).
 
-  Definition visited_coherent (m : state_mapg_type) (d : done_mapg_type) : Prop :=
-    ∀ γ, d !! γ ≠ None →
-      ∃ n, m !! γ = Some (done_val n) ∨ m !! γ = Some (finished_val n).
-
-  (** [done_id_coherent m d] strengthens [visited_coherent] by linking the
-      id-tag in [d] to the id-tag in [m]. Used in
-      [id_token_visit_reached_done_invalid] to derive the matching id from
-      a [visit_reached_done γ id] fragment. *)
+  (** [done_id_coherent m d] links the id-tag in [d] to the id-tag in [m]:
+      whenever [d !! γ ≡ Some (to_agree n)], [m !! γ] is in the matching
+      done/finished state at the same [n]. This subsumes the earlier
+      existence-style coherence — given [✓ d], every valid agree element
+      is equivalent to some [to_agree n] (cf. [to_agree_uninj]); see
+      [done_id_visited_coherent] below. *)
   Definition done_id_coherent (m : state_mapg_type) (d : done_mapg_type) : Prop :=
     ∀ γ n, d !! γ ≡ Some (to_agree n) →
       m !! γ = Some (done_val n) ∨ m !! γ = Some (finished_val n).
+
+  (** Derives the existence-style coherence (every key in [dom d] is
+      done/finished in [m] for some [n]) from [done_id_coherent] and [✓ d].
+      Used wherever the old [visited_coherent] hypothesis was needed. *)
+  Local Lemma done_id_visited_coherent m d :
+    ✓ d → done_id_coherent m d →
+      ∀ γ, d !! γ ≠ None →
+        ∃ n, m !! γ = Some (done_val n) ∨ m !! γ = Some (finished_val n).
+  Proof.
+    intros Hvd Hdid γ Hdγ.
+    destruct (d !! γ) as [xd|] eqn:Heqd; [|done].
+    assert (d !! γ ≡ Some xd) as Hxd by (rewrite Heqd; done).
+    assert (✓ xd) as Hvxd by (eapply lookup_valid_Some; [exact Hvd|exact Hxd]).
+    apply to_agree_uninj in Hvxd as [n Hxd_eq].
+    exists n. apply (Hdid γ n). rewrite Hxd. by f_equiv.
+  Qed.
 
   Definition pending_coherent (m : state_mapg_type) (ps : pending_setg_type) (pending_n : nat) : Prop :=
     pending_n = size ps ∧
@@ -83,8 +97,7 @@ Section visited_map_res.
     own pending_set_name (● GSet ps) ∗ pencount_frag pending_n ∗
     own pending_id_name (◯ GSet B) ∗
     ⌜∀ γ n, m !! γ = Some (done_val n) ∨ m !! γ = Some (finished_val n) → n ∈ B⌝ ∗
-    ⌜done_id_coherent m d⌝ ∗
-    ⌜visited_coherent m d⌝ ∗ ⌜pending_coherent m ps pending_n⌝.
+    ⌜done_id_coherent m d⌝ ∗ ⌜pending_coherent m ps pending_n⌝.
 
   Definition visited_map_update_pending
       (m : state_mapg_type) (d : done_mapg_type) (ps : pending_setg_type) pn (γs : gset gname) (B : gset nat) : iProp Σ :=
@@ -96,7 +109,6 @@ Section visited_map_res.
     own pending_id_name (◯ GSet B) ∗
     ⌜∀ γ n, m' !! γ = Some (done_val n) ∨ m' !! γ = Some (finished_val n) → n ∈ B⌝ ∗
     ⌜done_id_coherent m' d⌝ ∗
-    ⌜visited_coherent m' d⌝ ∗
     ⌜pending_coherent m' ps' (pn + size γs)⌝.
 
   Definition visited_map_update_done
@@ -107,7 +119,6 @@ Section visited_map_res.
     own pending_id_name (◯ GSet (B ∪ {[n]})) ∗
     ⌜∀ γ' n', <[ γ := done_val n ]>m !! γ' = Some (done_val n') ∨ <[ γ := done_val n ]>m !! γ' = Some (finished_val n') → n' ∈ B ∪ {[n]}⌝ ∗
     ⌜done_id_coherent (<[ γ := done_val n ]>m) (<[ γ := to_agree n ]>d)⌝ ∗
-    ⌜visited_coherent (<[ γ := done_val n ]>m) (<[ γ := to_agree n ]>d)⌝ ∗
     ⌜pending_coherent (<[ γ := done_val n ]>m) ps pn⌝.
 
   Definition visited_map_update_finished
@@ -118,7 +129,6 @@ Section visited_map_res.
     own pending_id_name (◯ GSet B) ∗
     ⌜∀ γ' n', <[ γ := finished_val n ]>m !! γ' = Some (done_val n') ∨ <[ γ := finished_val n ]>m !! γ' = Some (finished_val n') → n' ∈ B⌝ ∗
     ⌜done_id_coherent (<[ γ := finished_val n ]>m) d⌝ ∗
-    ⌜visited_coherent (<[ γ := finished_val n ]>m) d⌝ ∗
     ⌜pending_coherent (<[ γ := finished_val n ]>m) ps pn⌝.
 
   Definition visited_mapg_pending_removed (m : state_mapg_type) (d : done_mapg_type) (ps : pending_setg_type) (pending_n : nat) (γs : gset gname) (B : gset nat) : iProp Σ :=
@@ -127,7 +137,6 @@ Section visited_map_res.
     own pending_id_name (◯ GSet B) ∗
     ⌜∀ γ n, m !! γ = Some (done_val n) ∨ m !! γ = Some (finished_val n) → n ∈ B⌝ ∗
     ⌜done_id_coherent m d⌝ ∗
-    ⌜visited_coherent m d⌝ ∗
     ⌜pending_coherent m (ps ∖ γs) (pending_n - size γs)⌝.
 
   Lemma visited_map_update_pending_rewrite m d ps pn γs B:
@@ -288,7 +297,7 @@ Section visited_map_res.
         visited_map_update_pending m d ps pn {[γ]} B ∗ pencount_frag (pn+1) ∗
           visit_pending γ ∗ penset_frag {[γ]}.
   Proof.
-    iIntros "((Hms & Hd & Hps & Hpn1 & Hbag & %HBcoh & %Hdid & %Hcoh & %Hpcoh) & Hpn2)".
+    iIntros "((Hms & Hd & Hps & Hpn1 & Hbag & %HBcoh & %Hdid & %Hpcoh) & Hpn2)".
     set (γ := fresh (dom m ∪ ps)).
     assert (γ ∉ (dom m ∪ ps : gset gname)) as Hfr by apply is_fresh.
     rewrite not_elem_of_union in Hfr.
@@ -304,7 +313,7 @@ Section visited_map_res.
     rewrite /visited_map_update_pending /visit_pending /penset_frag.
     rewrite set_fold_singleton size_singleton (union_comm_L ps {[γ]}) /=.
     iFrame "Hms' Hd Hps' Hpn1 Hp Hpsf Hpn2 Hbag".
-    iPureIntro. split; last split; last split.
+    iPureIntro. split; last split.
     - intros γ' n' Hmγ'.
       destruct Hmγ' as [Hmγ' | Hmγ'];
         apply lookup_insert_Some in Hmγ' as [[<- Heq]|[Hne Hm']].
@@ -317,9 +326,6 @@ Section visited_map_res.
         destruct Hdid as [Hmγ | Hmγ]; rewrite Hfm in Hmγ; discriminate.
       + destruct (Hdid γ' n' Hdγ') as [Hmγ | Hmγ];
           [left|right]; rewrite lookup_insert_ne; done.
-    - intros γ' Hdγ'. destruct (decide (γ' = γ)) as [-> | Hne].
-      + destruct (Hcoh γ Hdγ') as (n & [Heq | Heq]); rewrite Hfm in Heq; discriminate.
-      + rewrite lookup_insert_ne; [|done]. by apply Hcoh.
     - destruct Hpcoh as [Hsize Hl]. split.
       + rewrite size_union; last set_solver. rewrite size_singleton. lia.
       + intros γ' Hγ'. destruct (decide (γ' = γ)) as [-> | Hne].
@@ -333,7 +339,7 @@ Section visited_map_res.
     visited_mapg_auth m d ps pn B -∗ visit_pending γ -∗ id_token n
     ==∗ visited_map_update_done m d ps pn γ n B ∗ visit_done γ n.
   Proof.
-    iIntros (Hdγ) "(Hms & Hd & Hps & Hpn & Hbag & %HBcoh & %Hdid & %Hcoh & %Hpcoh) H1 Htok".
+    iIntros (Hdγ) "(Hms & Hd & Hps & Hpn & Hbag & %HBcoh & %Hdid & %Hpcoh) H1 Htok".
     rewrite /visited_map_update_done /visit_done /visit_reached_done /id_token.
     iMod (own_update_2 _ _ _
       (● <[γ := done_val n]>m ⋅ ◯ {[γ := done_val n]})
@@ -351,7 +357,7 @@ Section visited_map_res.
     iAssert (own pending_id_name (◯ GSet (B ∪ {[n]})))%I with "[Hbag Htok]" as "Hbag'".
     { rewrite -gset_disj_union // auth_frag_op own_op. iFrame. }
     iModIntro.
-    iFrame "Hps Hpn Hf Hbag'". iPureIntro. split; last split; last split.
+    iFrame "Hps Hpn Hf Hbag'". iPureIntro. split; last split.
     - intros γ' n' Hmγ'.
       destruct Hmγ' as [Hmγ' | Hmγ'];
         apply lookup_insert_Some in Hmγ' as [[<- Heq]|[Hne Hm']].
@@ -367,10 +373,6 @@ Section visited_map_res.
       + rewrite lookup_insert_ne in Hdγ'; [|done].
         destruct (Hdid γ' n' Hdγ') as [Hmγ | Hmγ];
           [left|right]; rewrite lookup_insert_ne; done.
-    - intros γ' Hdγ'. destruct (decide (γ' = γ)) as [-> | Hne].
-      + exists n. left. by rewrite lookup_insert.
-      + rewrite lookup_insert_ne; [|done]. apply Hcoh.
-        rewrite lookup_insert_ne in Hdγ'; done.
     - destruct Hpcoh as [Hsize Hl]. split; [exact Hsize|].
       intros γ' Hγ'. destruct (decide (γ' = γ)) as [-> | Hne].
       + exfalso. rewrite lookup_insert in Hγ'.
@@ -383,7 +385,7 @@ Section visited_map_res.
     visited_mapg_auth m d ps pn B -∗ visit_done γ n
     ==∗ visited_map_update_finished m d ps pn γ n B ∗ visit_finished γ n.
   Proof.
-    iIntros "(Hms & Hd & Hps & Hpn & Hbag & %HBcoh & %Hdid & %Hcoh & %Hpcoh) [Hsfrag #Hreached]".
+    iIntros "(Hms & Hd & Hps & Hpn & Hbag & %HBcoh & %Hdid & %Hpcoh) [Hsfrag #Hreached]".
     rewrite /visited_map_update_finished /visit_finished /visit_reached_done.
     (* Derive m !! γ = Some (done_val n) from Hms ⋅ Hsfrag, using exclusivity of done_val. *)
     iDestruct (own_valid_2 with "Hms Hsfrag") as %Hvm.
@@ -404,7 +406,7 @@ Section visited_map_res.
       apply (exclusive_local_update _ (finished_val n)). done. }
     iFrame "Hd Hps Hpn Hreached Hbag". iPureIntro.
     assert (n ∈ B) as HnB by (apply (HBcoh γ n); by left).
-    split; last split; last split.
+    split; last split.
     - intros γ' n' Hmγ'.
       destruct Hmγ' as [Hmγ' | Hmγ'];
         apply lookup_insert_Some in Hmγ' as [[<- Heq]|[Hne Hm']].
@@ -423,9 +425,6 @@ Section visited_map_res.
         subst n. right. by rewrite lookup_insert.
       + rewrite lookup_insert_ne; [|done].
         destruct (Hdid γ' n' Hdγ') as [Hmγ | Hmγ]; [by left|by right].
-    - intros γ' Hdγ'. destruct (decide (γ' = γ)) as [-> | Hne].
-      + exists n. right. by rewrite lookup_insert.
-      + rewrite lookup_insert_ne; [|done]. by apply Hcoh.
     - destruct Hpcoh as [Hsize Hl]. split; [exact Hsize|].
       intros γ' Hγ'. destruct (decide (γ' = γ)) as [-> | Hne].
       + exfalso. rewrite lookup_insert in Hγ'.
@@ -491,7 +490,7 @@ Section visited_map_res.
     d !! γ = Some (to_agree n) →
     visited_mapg_auth m d ps pn B ==∗ visited_mapg_auth m d ps pn B ∗ visit_reached_done γ n.
   Proof.
-    iIntros (Hd) "(Hms & Hd & Hps & Hpn & Hbag & %HBcoh & %Hdid & %Hcoh & %Hpcoh)".
+    iIntros (Hd) "(Hms & Hd & Hps & Hpn & Hbag & %HBcoh & %Hdid & %Hpcoh)".
     rewrite /visit_reached_done.
     iMod (own_update _ _ (● d ⋅ ◯ {[γ := to_agree n]}) with "Hd") as "[Hd #Hr]".
     { apply auth_update_dfrac_alloc; [apply _|].
@@ -503,14 +502,17 @@ Section visited_map_res.
   Lemma visited_reached_done_invalid γ n m d ps pn B :
     visited_mapg_auth m d ps pn B -∗ visit_reached_done γ n -∗ visit_pending γ -∗ False.
   Proof.
-    iIntros "(Hms & Hd & Hps & Hpn & Hbag & %HBcoh & %Hdid & %Hcoh & %Hpcoh) Hreached Hpending".
+    iIntros "(Hms & Hd & Hps & Hpn & Hbag & %HBcoh & %Hdid & %Hpcoh) Hreached Hpending".
     rewrite /visit_reached_done /visit_pending.
     iDestruct (own_valid_2 with "Hd Hreached") as %Hvd.
-    apply auth_both_valid_discrete in Hvd as [Hincl_d _].
-    apply singleton_included_l in Hincl_d as (xd & Hxd & _).
-    assert (d !! γ ≠ None) as Hdγ.
-    { intros Heq. rewrite Heq in Hxd. inversion Hxd. }
-    destruct (Hcoh γ Hdγ) as (n' & Hmγ).
+    apply auth_both_valid_discrete in Hvd as [Hincl_d Hvalid_d].
+    apply singleton_included_l in Hincl_d as (xd & Hxd & Hle_d).
+    assert (✓ xd) as Hvxd
+      by (eapply lookup_valid_Some; [exact Hvalid_d|exact Hxd]).
+    assert (d !! γ ≡ Some (to_agree n)) as Hdg_eq.
+    { rewrite Hxd. f_equiv. apply Some_included in Hle_d as [|Hinc]; [by symmetry|].
+      symmetry. by apply (agree_valid_included _ _ Hvxd). }
+    pose proof (Hdid γ n Hdg_eq) as Hmγ.
     iDestruct (own_valid_2 with "Hms Hpending") as %Hvm.
     apply auth_both_valid_discrete in Hvm as [Hincl_m _].
     apply singleton_included_l in Hincl_m as (ym & Hym & Hle).
@@ -523,7 +525,7 @@ Section visited_map_res.
       apply csum_included in Hle as [Hbot | [(?&?& Heq1 & Heq2 & Hinc) | (?&?& Heq1 & _ & _)]].
       + by inversion Hbot.
       + injection Heq1 as <-. injection Heq2 as <-.
-        exfalso. apply (exclusive_included (Excl None) (Excl (Some n'))); done.
+        exfalso. apply (exclusive_included (Excl None) (Excl (Some n))); done.
       + by inversion Heq1.
     - rewrite /pending_val /finished_val in Heq. by inversion Heq.
     - rewrite /pending_val /finished_val in Hle.
@@ -565,14 +567,23 @@ Section visited_map_res.
     ([∗ set] γ ∈ γs, ∃ n, visit_reached_done γ n) ==∗
     visited_mapg_pending_removed m d ps pn γs B ∗ pencount_frag (pn - size γs).
   Proof.
-    iIntros "(Hms & Hd & Hps & Hpn1 & Hbag & %HBcoh & %Hdid & %Hcoh & %Hpcoh) Hpn2 Hfrag #Hreached".
-    iAssert (⌜∀ γ, γ ∈ γs → d !! γ ≠ None⌝)%I as %Hdγs.
+    iIntros "(Hms & Hd & Hps & Hpn1 & Hbag & %HBcoh & %Hdid & %Hpcoh) Hpn2 Hfrag #Hreached".
+    iAssert (⌜∀ γ, γ ∈ γs →
+              ∃ n, m !! γ = Some (done_val n) ∨ m !! γ = Some (finished_val n)⌝)%I
+      as %Hmγs.
     { iIntros (γ Hin).
       iDestruct (big_sepS_elem_of with "Hreached") as (n) "Hr"; first done.
-      iDestruct (own_valid_2 with "Hd Hr") as %Hv.
-      apply auth_both_valid_discrete in Hv as [Hincl _].
-      apply singleton_included_l in Hincl as (xd & Hxd & _).
-      iPureIntro. intros Heq. rewrite Heq in Hxd. inversion Hxd. }
+      rewrite /visit_reached_done.
+      iDestruct (own_valid_2 with "Hd Hr") as %Hvd.
+      apply auth_both_valid_discrete in Hvd as [Hincl Hvalid_d].
+      apply singleton_included_l in Hincl as (xd & Hxd & Hle).
+      iPureIntro.
+      assert (✓ xd) as Hvxd
+        by (eapply lookup_valid_Some; [exact Hvalid_d|exact Hxd]).
+      assert (d !! γ ≡ Some (to_agree n)) as Hdg_eq.
+      { rewrite Hxd. f_equiv. apply Some_included in Hle as [|Hinc]; [by symmetry|].
+        symmetry. by apply (agree_valid_included _ _ Hvxd). }
+      exists n. apply (Hdid γ n Hdg_eq). }
     rewrite /visited_mapg_pending_removed /penset_frag.
     iCombine "Hps Hfrag" as "Hpsfull".
     iDestruct (own_valid with "Hpsfull") as %Hv.
@@ -581,14 +592,14 @@ Section visited_map_res.
     { apply auth_update_dealloc, gset_disj_dealloc_local_update. }
     iMod (pn_update pn (pn - size γs) with "Hpn1 Hpn2") as "[Hpn1 Hpn2]".
     iModIntro. iFrame "Hms Hd Hps' Hpn1 Hpn2 Hbag". iPureIntro.
-    split; [exact HBcoh|]. split; [exact Hdid|]. split; first done.
+    split; [exact HBcoh|]. split; [exact Hdid|].
     destruct Hpcoh as [Hsz Hpcoh].
     split.
     - rewrite (size_difference _ _ Hincl) -Hsz //.
     - intros γ' Hm. specialize (Hpcoh γ' Hm).
       destruct (decide (γ' ∈ γs)) as [Hin | Hnin].
-      + exfalso. specialize (Hdγs _ Hin).
-        destruct (Hcoh γ' Hdγs) as (n & [Hmγ | Hmγ]); rewrite Hmγ in Hm;
+      + exfalso. destruct (Hmγs _ Hin) as (n & [Hmγ | Hmγ]);
+          rewrite Hmγ in Hm;
           rewrite /done_val /finished_val /pending_val in Hm;
           by inversion Hm.
       + by apply elem_of_difference.
@@ -603,7 +614,7 @@ Section visited_map_res.
           m !! γ ≠ Some (finished_val id)⌝ ∗
       visited_mapg_auth m d ps pn B ∗ id_token id.
   Proof.
-    iIntros "(Hms & Hd & Hps & Hpn & Hbag & %HBcoh & %Hdid & %Hcoh & %Hpcoh) Htok".
+    iIntros "(Hms & Hd & Hps & Hpn & Hbag & %HBcoh & %Hdid & %Hpcoh) Htok".
     iAssert (⌜id ∉ B⌝)%I as %HnotB.
     { rewrite /id_token. iDestruct (own_valid_2 with "Hbag Htok") as %Hv.
       rewrite auth_frag_op_valid gset_disj_valid_op in Hv. iPureIntro. set_solver. }
@@ -619,7 +630,7 @@ Section visited_map_res.
   Proof.
     iIntros "Hauth Htok Hreached".
     iDestruct "Hauth" as
-      "(Hms & Hd & Hps & Hpn & Hbag & %HBcoh & %Hdid & %Hcoh & %Hpcoh)".
+      "(Hms & Hd & Hps & Hpn & Hbag & %HBcoh & %Hdid & %Hpcoh)".
     rewrite /id_token /visit_reached_done.
     (* id ∉ B *)
     iDestruct (own_valid_2 with "Hbag Htok") as %Hv.
